coq/TypedChoreography.v
@@ -8,17 +8,17 @@ Module TypedChoreography (L : Locations) (E : Expression) (TE : TypedExpression 
   Include (Choreography E L).
 
   Reserved Notation "G ;; D ⊢c C ::: tau @ p" (at level 30).
-  Inductive ctyping : (L.t -> nat -> ExprTyp) -> (nat -> L.t * ExprTyp) -> Chor -> ExprTyp -> L.t -> Prop :=
-  | TDone : forall (Γ : L.t -> nat -> ExprTyp) (Δ : nat -> L.t * ExprTyp)
-              (p : L.t) (e : Expr) (tau : ExprTyp),
+  Inductive ctyping : (Loc -> nat -> ExprTyp) -> (nat -> Loc * ExprTyp) -> Chor -> ExprTyp -> Loc -> Prop :=
+  | TDone : forall (Γ : Loc -> nat -> ExprTyp) (Δ : nat -> Loc * ExprTyp)
+              (p : Loc) (e : Expr) (tau : ExprTyp),
        (Γ p) ⊢e e ::: tau ->
   (* ------------------------------ *)
-      Γ ;; Δ ⊢c CDone p e ::: tau @ p
-  | TVar : forall (Γ : L.t -> nat -> ExprTyp) (Δ : nat -> L.t * ExprTyp) (n : nat),
+      Γ ;; Δ ⊢c Done p e ::: tau @ p
+  | TVar : forall (Γ : Loc -> nat -> ExprTyp) (Δ : nat -> Loc * ExprTyp) (n : nat),
   (* ----------------------------- *)
-      Γ ;; Δ ⊢c CVar n ::: snd (Δ n) @ fst (Δ n)
-  | TSend : forall (Γ : L.t -> nat -> ExprTyp) (Δ : nat -> L.t * ExprTyp)
-              (p : L.t) (e : Expr) (τ : ExprTyp) (q : L.t) (C : Chor) (r : L.t) (sigma : ExprTyp),
+      Γ ;; Δ ⊢c Var n ::: snd (Δ n) @ fst (Δ n)
+  | TSend : forall (Γ : Loc -> nat -> ExprTyp) (Δ : nat -> Loc * ExprTyp)
+              (p : Loc) (e : Expr) (τ : ExprTyp) (q : Loc) (C : Chor) (r : Loc) (sigma : ExprTyp),
       (Γ p) ⊢e e ::: τ ->
       (fun r n => if L.eq_dec q r
                then match n with
@@ -28,16 +28,33 @@ Module TypedChoreography (L : Locations) (E : Expression) (TE : TypedExpression 
                else Γ r n);; Δ ⊢c C ::: sigma @ r ->
       p <> q ->
   (* --------------------------------------- *)
-      Γ ;; Δ ⊢c (CSend p e q C) ::: sigma @ r
-  | TIf : forall (Γ : L.t -> nat -> ExprTyp) (Δ : nat -> L.t * ExprTyp)
-            (p : L.t) (e : Expr) (C1 C2 : Chor) (q : L.t) (tau : ExprTyp),
+      Γ ;; Δ ⊢c (Send p e q C) ::: sigma @ r
+  | TIf : forall (Γ : Loc -> nat -> ExprTyp) (Δ : nat -> Loc * ExprTyp)
+            (p : Loc) (e : Expr) (C1 C2 : Chor) (q : Loc) (tau : ExprTyp),
       (Γ p) ⊢e e ::: bool ->
       Γ ;; Δ ⊢c C1 ::: tau @ q ->
       Γ ;; Δ ⊢c C2 ::: tau @ q ->
   (* --------------------------------- *)
-      Γ;; Δ ⊢c CIf p e C1 C2 ::: tau @ q
-  | TDef : forall (Γ : L.t -> nat -> ExprTyp) (Δ : nat -> L.t * ExprTyp)
-             (C1 C2 : Chor) (p q : L.t) (τ σ : ExprTyp),
+      Γ;; Δ ⊢c If p e C1 C2 ::: tau @ q
+  | TSync : forall (Γ : Loc -> nat -> ExprTyp) (Δ : nat -> Loc * ExprTyp)
+              (p : Loc) (d : LRChoice) (q : Loc) (C : Chor) (τ : ExprTyp) (r : Loc),
+      Γ ;; Δ ⊢c C ::: τ @ r ->
+  (* ---------------------------------- *)
+      Γ ;; Δ ⊢c Sync p d q C ::: τ @ r
+  | TDefLocal : forall (Γ : Loc -> nat -> ExprTyp) (Δ : nat -> Loc * ExprTyp)
+                  (p : Loc) (C1 C2 : Chor) (τ σ : ExprTyp) (q : Loc),
+      Γ ;; Δ ⊢c C1 ::: τ @ p ->
+      (fun r n =>
+         if L.eq_dec p r
+         then match n with
+              | 0 => τ
+              | S n => Γ r n
+              end
+         else Γ r n);; Δ ⊢c C2 ::: σ @ q ->
+  (* ------------------------------------*)
+      Γ ;; Δ ⊢c DefLocal p C1 C2 ::: σ @ q
+  | TDefGlobal : forall (Γ : Loc -> nat -> ExprTyp) (Δ : nat -> Loc * ExprTyp)
+                   (C1 C2 : Chor) (p q : Loc) (τ σ : ExprTyp),
       Γ;; (fun n =>
             match n with
             | 0 => (q, σ)
@@ -49,233 +66,239 @@ Module TypedChoreography (L : Locations) (E : Expression) (TE : TypedExpression 
             | S n => Δ n
             end) ⊢c C2 ::: τ @ p ->
   (* ---------------------------------------- *)
-      Γ;; Δ ⊢c CDef C1 C2 ::: τ @ p
+      Γ;; Δ ⊢c DefGlobal C1 C2 ::: τ @ p
   where "Gamma ;; Delta ⊢c C ::: tau @ p" := (ctyping Gamma Delta C tau p).
   Hint Constructors ctyping : Chor.
 
 
-  Theorem ChorWeakening : forall (Γ1 Γ2 : L.t -> nat -> ExprTyp) (Δ1 Δ2 : nat -> L.t * ExprTyp)
-                            (ξe : L.t -> nat -> nat) (ξc : nat -> nat),
-      (forall p n, Γ1 p n = Γ2 p (ξe p n)) ->
-      (forall n, Δ1 n = Δ2 (ξc n)) ->
-      forall (τ : ExprTyp) (r : L.t) (C : Chor),
-        Γ1;; Δ1 ⊢c C ::: τ @ r ->
-        Γ2;; Δ2 ⊢c C⟨c| ξc; ξe⟩ ::: τ @ r.
-  Proof.
-    intros Γ1 Γ2 Δ1 Δ2 ξe ξc subΓ subΔ τ r C; revert Γ1 Γ2 Δ1 Δ2 ξe ξc subΓ subΔ τ r;
-      ChorInduction C; intros Γ1 Γ2 Δ1 Δ2 ξe ξc subΓ subΔ τ r typing; simpl; inversion typing.
-    - apply TDone. apply ExprWeakening with (Γ := Γ1 p).
-      rewrite <- H4; apply subΓ.
-      rewrite H4; auto.
-    - rewrite subΔ. apply TVar; auto.
-    - inversion typing.
-      rewrite <- H4 in *; subst.
-      unfold ChorUpExprRename. unfold ExprUpRename.
-      rename τ0 into σ; apply TSend with (τ := σ);
-        [apply ExprWeakening with (Γ := Γ1 p); auto| |]; auto.
-      apply IHC with (Γ1 := fun (r : L.t) (n : nat) => if L.eq_dec q r then match n with
-                                                                         | 0 => σ
-                                                                         |S n0 => Γ1 r n0
-                                                                         end
-                                                  else Γ1 r n) (Δ1 := Δ1); auto.
-      intros s n.
-      destruct (L.eq_dec q s); simpl.
-      destruct n; auto.
-      auto.
-    - apply TIf; [eapply ExprWeakening; eauto | eapply IHC0; eauto | eapply IHC1; eauto].
-    - eapply TDef. eapply IHC0; eauto.
-      intro n; simpl. unfold ChorUpRename. destruct n; auto.
-      eapply IHC1; eauto.
-      intro n; simpl. unfold ChorUpRename. destruct n; auto.
+  Theorem TypeExprWeakening : forall (Γ1 Γ2 : Loc -> nat -> ExprTyp) (Δ : nat -> Loc * ExprTyp)
+                               (ξ : Loc -> nat -> nat),
+      (forall p n, Γ1 p n = Γ2 p (ξ p n)) ->
+      forall (τ : ExprTyp) (p : Loc) (C : Chor),
+        Γ1;; Δ ⊢c C ::: τ @ p ->
+        Γ2;; Δ ⊢c C⟨ce| ξ⟩ ::: τ @ p.
+  Proof using.
+    intros Γ1 Γ2 Δ ξ eqv τ p C typing; revert Γ2 ξ eqv; induction typing; intros Γ2 ξ eqv;
+      cbn; repeat match goal with
+                  | [ H : ?Γ ?p ⊢e ?e ::: ?t, eqv : forall p n, ?Γ p n = ?Γ2 p (?ξ p n) |- _] =>
+                    lazymatch goal with
+                    | [_ : Γ2 p ⊢e e ⟨e| ξ p ⟩ ::: t |- _ ] => fail
+                    | _ => pose proof (ExprWeakening (Γ p) (Γ2 p) (ξ p) e t (eqv p) H)
+                    end
+                  end; auto with Chor.
+    - apply TSend with (τ := τ); auto; apply IHtyping.
+      intros p0 n; unfold ChorUpExprRename; unfold ExprUpRename;
+        destruct (L.eq_dec q p0); destruct n; auto.
+    - apply TDefLocal with (τ := τ); auto; apply IHtyping2.
+      intros p0 n; unfold ChorUpExprRename; unfold ExprUpRename;
+        destruct (L.eq_dec p p0); destruct n; auto.
+    - apply TDefGlobal with (q := q) (σ := σ); auto.
+  Qed.
+      
+  Theorem TypeChorWeakening : forall (Γ : Loc -> nat -> ExprTyp) (Δ1 Δ2 : nat -> Loc * ExprTyp)
+                                (ξ : nat -> nat),
+      (forall n, Δ1 n = Δ2 (ξ n)) ->
+      forall (τ : ExprTyp) (p : Loc) (C : Chor),
+        Γ ;; Δ1 ⊢c C ::: τ @ p ->
+        Γ ;; Δ2 ⊢c C ⟨c| ξ⟩ ::: τ @ p.
+  Proof using.
+    intros Γ Δ1 Δ2 ξ eqv τ p C typing; revert Δ2 ξ eqv; induction typing;
+      intros Δ2 ξ eqv; cbn; eauto with Chor.
+    - rewrite eqv; apply TVar.
+    - apply TDefGlobal with (q := q) (σ := σ); auto with Chor.
+      apply IHtyping1; intro n; unfold ChorUpRename; destruct n; auto.
+      apply IHtyping2; intro n; unfold ChorUpRename; destruct n; auto.
   Qed.
   
-  Theorem ChorTypingExt : forall (Γ1 Γ2 : L.t -> nat -> ExprTyp) (Δ1 Δ2 : nat -> L.t * ExprTyp)
-                            (C : Chor) (p : L.t) (τ : ExprTyp),
-      (forall (p : L.t) (n : nat), Γ1 p n = Γ2 p n) ->
+  Theorem ChorTypingExt : forall (Γ1 Γ2 : Loc -> nat -> ExprTyp) (Δ1 Δ2 : nat -> Loc * ExprTyp)
+                            (C : Chor) (p : Loc) (τ : ExprTyp),
+      (forall (p : Loc) (n : nat), Γ1 p n = Γ2 p n) ->
       (forall n : nat, Δ1 n = Δ2 n) ->
       Γ1;; Δ1 ⊢c C ::: τ @ p -> Γ2;; Δ2 ⊢c C ::: τ @ p.
   Proof.
-    intros Γ1 Γ2 Δ1 Δ2 C p τ eqΓ eqΔ typing; revert Γ1 Γ2 Δ1 Δ2 p τ eqΓ eqΔ typing;
-      ChorInduction C; intros Γ1 Γ2 Δ1 Δ2 r τ eqΓ eqΔ typing.
-    - inversion typing; apply TDone.
-      apply ExprTypingExt with (Γ := Γ1 r); auto.
-    - inversion typing. rewrite eqΔ; apply TVar.
-    - inversion typing. apply TSend with (τ := τ0); [eapply ExprTypingExt; eauto | |auto].
-      eapply IHC; [| auto | exact H8]; subst.
-      intros p3 n; simpl. destruct (L.eq_dec q p3); auto.
-      destruct n; auto.
-    - inversion typing; subst.
-      apply TIf; [eapply ExprTypingExt; eauto| eapply IHC0 | eapply IHC1]; eauto.
-    - inversion typing; subst.
-      eapply TDef; [eapply IHC0 | eapply IHC1].
-      3: exact H3.
-      all: eauto.
-      all: intro n; simpl; destruct n; auto.
+    intros Γ1 Γ2 Δ1 Δ2 C p τ eqΓ eqΔ typing; revert Γ2 Δ2 eqΓ eqΔ; induction typing;
+      intros Γ2 Δ2 eqΓ eqΔ;
+      repeat match goal with
+             | [ H : ?Γ ?p ⊢e ?e ::: ?t, eqv : forall p n, ?Γ p n = ?Γ2 p n |- _ ] =>
+               lazymatch goal with
+               | [_ : Γ2 p ⊢e e ::: t |- _ ] => fail
+               | _ => pose proof (ExprTypingExt (Γ p) (Γ2 p) e t (eqv p) H)
+               end
+             end; auto with Chor.
+    - rewrite eqΔ; auto with Chor.
+    - apply TSend with (τ := τ); auto with Chor; apply IHtyping; auto.
+      intros p0 n; destruct (L.eq_dec q p0); destruct n; auto.
+    - apply TDefLocal with (τ := τ); auto with Chor; apply IHtyping2; auto.
+      intros p0 n; destruct (L.eq_dec p p0); destruct n; auto.
+    - apply TDefGlobal with (q := q) (σ := σ); auto with Chor;
+        [apply IHtyping1 | apply IHtyping2]; auto; intro n; destruct n; auto.
   Qed.
 
-  Definition ChorSubstTyping Γ1 Δ1 σc σe Γ2 Δ2 :=
-    (forall n : nat, Γ2;; Δ2 ⊢c (σc n) ::: (snd (Δ1 n)) @ (fst (Δ1 n))) /\
-    (forall p : L.t, (Γ1 p) ⊢es (σe p) ⊣ (Γ2 p)).
+  Definition ChorSubstTyping Γ Δ1 σ Δ2 :=
+    (forall (n : nat), Γ;; Δ2 ⊢c (σ n) ::: (snd (Δ1 n)) @ (fst (Δ1 n))).
 
-  Theorem ChorSubstTypingSpec : forall Γ1 Δ1 σc σe Γ2 Δ2,
-      (ChorSubstTyping Γ1 Δ1 σc σe Γ2 Δ2) -> forall (C : Chor) (τ : ExprTyp) (p : L.t),
-          (Γ1;; Δ1 ⊢c C ::: τ @ p) -> (Γ2;; Δ2 ⊢c (C [c| σc; σe]) ::: τ @ p).
+  Theorem ChorExprSubstTypingSpec : forall Γ1 σ Γ2 Δ C p τ,
+      (forall q, Γ1 q ⊢es σ q ⊣ Γ2 q) -> Γ1 ;; Δ ⊢c C ::: τ @ p -> Γ2 ;; Δ ⊢c C [ce| σ] ::: τ @ p.
+  Proof using.
+    intros Γ1 σ Γ2 Δ C p τ eqv typing; revert σ Γ2 eqv; induction typing; intros σ' Γ2 eqv;
+      cbn; repeat match goal with
+                  | [ H : ?Γ ?p ⊢e ?e ::: ?t, eqv : forall q, ?Γ q ⊢es ?σ' q ⊣ ?Γ2 q |- _] =>
+                    lazymatch goal with
+                    | [ _ : Γ2 p ⊢e e [e|σ' p] ::: t |- _] => fail
+                    | _ => pose proof (ExprSubstType (Γ p) (Γ2 p) (σ' p) e t (eqv p) H)
+                    end
+                  end; eauto with Chor.
+    - apply TSend with (τ := τ); auto; apply IHtyping.
+      intro q0; unfold ExprSubstTyping; intro n; unfold ChorUpExprSubst;
+        destruct (L.eq_dec q q0); destruct n; auto.
+      apply ExprVarTyping. apply ExprWeakening with (Γ := Γ2 q0); auto.
+      all: apply eqv.
+    - apply TDefLocal with (τ := τ); auto; apply IHtyping2; auto.
+      intro q0; unfold ChorUpExprSubst; intro n;
+        destruct (L.eq_dec p q0); destruct n; auto with Chor.
+      apply ExprVarTyping. apply ExprWeakening with (Γ := Γ2 q0); auto.
+      all: apply eqv.
+  Qed.      
+         
+
+  Lemma TypingLocalUp :forall Γ Δ C τ p,
+      Γ ;; Δ ⊢c C ::: τ @ p ->
+      forall q σ, (fun r n => if L.eq_dec r q
+                      then match n with
+                           | 0 => σ
+                           | S n => Γ r n
+                           end
+                      else Γ r n) ;; Δ ⊢c C ⟨ce| fun p n => if L.eq_dec q p then S n else n ⟩ ::: τ @ p.
+  Proof using.
+    intros Γ Δ C τ p H q σ.
+    apply TypeExprWeakening with (Γ1 := Γ); auto.
+    intros p0 n; destruct (L.eq_dec q p0); subst.
+    destruct (L.eq_dec p0 p0) as [_ | neq]; [|destruct (neq eq_refl)]; auto.
+    destruct (L.eq_dec p0 q) as [eq | _ ]; [destruct (n0 (eq_sym eq))|] ;auto.
+  Qed.
+  
+  Theorem ChorSubstTypingSpec : forall Γ Δ1 σ Δ2,
+      (ChorSubstTyping Γ Δ1 σ Δ2) ->
+      forall (C : Chor) (τ : ExprTyp) (p : Loc),
+        (Γ;; Δ1 ⊢c C ::: τ @ p) -> (Γ;; Δ2 ⊢c (C [c| σ]) ::: τ @ p).
   Proof.
-    intros Γ1 Δ1 σc σe Γ2 Δ2 substyping C;
-      revert Γ1 Δ1 σc σe Γ2 Δ2 substyping;
-      ChorInduction C;
-      intros Γ1 Δ1 σc σe Γ2 Δ2 substyping τ r typing; simpl.
-    all: unfold ChorSubstTyping in substyping; destruct substyping as [st1 st2].
-    all: inversion typing; subst.
-    - apply TDone; eapply ExprSubstType; eauto.
-    - apply st1.
-    - eapply TSend; auto. simpl. eapply ExprSubstType; eauto.
-      apply IHC with (Γ1 := fun r n => if L.eq_dec q r then match n with
-                                                          | 0 => τ0
-                                                          | S n0 => Γ1 r n0
-                                                          end else Γ1 r n)
-      (Δ1 := Δ1); [unfold ChorSubstTyping; split |]; auto.
-      -- intros n.
-         unfold SendUpChorSubst. eapply ChorWeakening; eauto.
-         intros p1 m; destruct (L.eq_dec q p1); reflexivity.
-      -- unfold ChorUpExprSubst. intro p2. eapply ExprSubstRWeakening.
-         intro n; reflexivity.
-         unfold ExprSubstTyping. intro n; simpl.
-         destruct (L.eq_dec q p2). destruct n. apply ExprVarTyping.
-         apply ExprWeakening with (Γ := Γ2 p2); auto.
-         apply st2. apply st2.
-    - apply TIf; 
-        [ eapply ExprSubstType; eauto | eapply IHC0; eauto | eapply IHC1; eauto];
-        unfold ChorSubstTyping; split; auto.
-
-    - eapply TDef; [eapply IHC0; eauto | eapply IHC1; eauto];
-        unfold ChorSubstTyping; split; eauto;
-          unfold ChorUpSubst.
-      all: intro n; destruct n; [apply TVar | eapply ChorWeakening; eauto].
+    intros Γ Δ1 σ Δ2 styping C τ p typing; revert σ Δ2 styping; induction typing;
+      try rename σ into ρ; intros σ Δ2 styping; cbn; auto with Chor.
+    - apply TSend with (τ := τ); auto. apply IHtyping.
+      unfold ChorSubstTyping. intro n. unfold ChorSubstTyping in styping.
+      unfold ChorUpSubstForExpr. apply TypeExprWeakening with (Γ1 := Γ); auto.
+      intros p0 n0; destruct (L.eq_dec q p0); auto.
+    - apply TDefLocal with (τ := τ). apply IHtyping1; auto.
+      unfold ChorUpSubstForExpr. apply IHtyping2. unfold ChorSubstTyping.
+      intro n; apply TypeExprWeakening with (Γ1 := Γ); auto.
+      intros p0 n0; destruct (L.eq_dec p p0); auto.
+    - apply TDefGlobal with (σ := ρ) (q := q); auto.
+      apply IHtyping1. unfold ChorSubstTyping; unfold ChorUpSubst.
+      intro n. destruct n. apply TVar. apply TypeChorWeakening with (Δ1 := Δ2); auto.
+      apply IHtyping2. unfold ChorSubstTyping; unfold ChorUpSubst.
+      intro n. destruct n. apply TVar. apply TypeChorWeakening with (Δ1 := Δ2); auto.
   Qed.
 
-  Lemma SendSubstTyping : forall (Γ : L.t -> nat -> ExprTyp) (Δ : nat -> L.t * ExprTyp)
-                            (p : L.t) (e : Expr) (τ : ExprTyp),
-      Γ p ⊢e e ::: τ ->
-      ChorSubstTyping (fun r n => if L.eq_dec p r
-                               then match n with
-                                    | 0 => τ
-                                    | S n => Γ r n
-                                    end
-                               else Γ r n) Δ ChorIdSubst (SendSubst p e) Γ Δ.
-  Proof.
-    intros Γ Δ p e τ typ.
-    unfold ChorSubstTyping; split; auto.
-    - intro n; unfold ChorIdSubst; auto with Chor.
-    - intro q. unfold ExprSubstTyping.
-      unfold SendSubst; destruct (L.eq_dec p q); intro m;
-        [rewrite <- e0; destruct m; auto|]; apply ExprVarTyping.
+  Lemma SendExprSubstTyping: forall (Γ : Loc -> nat -> ExprTyp) (p : Loc) (e : Expr) (τ : ExprTyp),
+      (Γ p ⊢e e ::: τ) ->
+      forall q, ((fun r n => if L.eq_dec p r
+                     then match n with
+                          | 0 => τ
+                          | S n => Γ r n
+                          end
+                     else Γ r n) q) ⊢es SendExprSubst p e q ⊣ (Γ q).
+  Proof using.
+    intros Γ p e τ tpng q. unfold SendExprSubst.
+    unfold ExprSubstTyping. intro n. destruct n; destruct (L.eq_dec p q); subst; auto.
+    all: apply ExprVarTyping.
   Qed.
 
-  Lemma DefSubstTyping : forall (Γ : L.t -> nat -> ExprTyp) (Δ : nat -> L.t * ExprTyp) (C : Chor)
-    (σ : ExprTyp) (p : L.t),
-      (Γ;; fun n =>
-            match n with
-            | 0 => (p, σ)
-            | S n => Δ n
-            end ⊢c C ::: σ @ p) ->
-      ChorSubstTyping Γ (fun n =>
-                           match n with
-                           | 0 => (p, σ)
-                           | S n => Δ n
-                           end) (DefSubst C) ExprChorIdSubst Γ Δ.
-  Proof.
-    intros Γ Δ C σ p H.
-    unfold ChorSubstTyping; split.
-    unfold DefSubst; intro n; destruct n; eauto with Chor.
-    intro p0; unfold ExprChorIdSubst. fold ExprIdSubst. apply ExprIdSubstTyping.
-  Qed.    
-
-  Theorem ChorEquiv'Typing : forall (C1 C2 : Chor),
-      C1 ≡' C2 ->
-      forall (Γ : L.t -> nat -> ExprTyp) (Δ : nat -> L.t * ExprTyp) (τ : ExprTyp) (p : L.t),
-        Γ;; Δ ⊢c C1 ::: τ @ p -> Γ;; Δ ⊢c C2 ::: τ @ p.
-  Proof.
-    intros C1 C2 equiv; induction equiv; intros Γ Δ τ Alice typ; auto with Chor.
-    - inversion typ. clear Γ0 H1 Δ0 H2 p0 H e0 H0 q0 H4 C H5 sigma H3 r H6.
-      rename τ0 into σ. rename H7 into ltyp. rename H8 into Ctyp.
-      apply TSend with (τ := σ); auto.
-    - inversion typ; apply TIf; auto.
-    - inversion typ; eapply TDef; eauto.
-    - inversion typ; clear Γ0 H5 Δ0 H6 p0 H3 e H4 q0 H8 C H9 sigma H7 r0 H10;
-        rename τ0 into σ; rename H11 into ltyp1; rename H12 into ContTyp1.
-      inversion ContTyp1. clear Γ0 H5 Δ0 H6 p0 H3 e H4 q0 H8 C H9 sigma H7 r0 H10;
-        rename H11 into ltyp2; rename H12 into ContTyp2; rename τ0 into ρ.
-      destruct (L.eq_dec q r) as [e | _]; [exfalso; apply H0; apply e | ].
-      apply TSend with (τ := ρ); [apply ltyp2 | |]; auto.
-      apply TSend with (τ := σ); auto.
-      -- destruct (L.eq_dec s p) as [e | _]; [exfalso; apply H1; symmetry; apply e |].
-         apply ltyp1.
-      -- apply IHequiv in ContTyp2. eapply ChorTypingExt; [ | | exact ContTyp2]; auto.
-         intros t n; simpl. destruct (L.eq_dec s t) as [e3 | n1].
-         destruct (L.eq_dec q t) as [e4 | n2]; [exfalso; apply H2; transitivity t; auto|].
-         destruct n; auto.
-         destruct (L.eq_dec q t); auto.
-    - inversion typ; clear Γ0 H4 Δ0 H5 p0 H1 e H2 C0 H3 C3 H7 tau H6 q0 H8;
-        rename H9 into ltyp1; rename H10 into Btyp11; rename H11 into Btyp21.
-      inversion Btyp11; clear Γ0 H3 Δ0 H4 p0 H1 e H2 q0 H6 C H7 sigma H5 r0 H8;
-        rename τ0 into σ; rename H9 into ltyp2; rename H10 into typC1.
-      inversion Btyp21; clear Γ0 H3 Δ0 H4 p0 H1 e H2 q0 H6 C H7 sigma H5 r0 H8;
-        rename τ0 into ρ; rename H9 into ltyp3; rename H10 into typC2.
-      apply TSend with (τ := σ); auto.
-      apply TIf; [| apply IHequiv1 in typC1; auto |].
-      destruct (L.eq_dec r p) as [eq | _ ]; [exfalso; apply H0; symmetry; exact eq| auto ].
-      rewrite (ExprTypingUnique _ _ _ _ ltyp2 ltyp3); apply IHequiv2 in typC2; auto.
-    - inversion typ; clear Γ0 H3 Δ0 H4 p0 H1 e H2 q0 H6 C H7 sigma H5 r0 H8;
-        rename τ0 into σ; rename H9 into ltyp1; rename H10 into typif.
-      inversion typif; clear Γ0 H4 Δ0 H5 p0 H1 e H2 C0 H3 C3 H7 tau H6 q0 H8;
-        rename H9 into ltyp2; rename H10 into typC1; rename H11 into typC2.
-      destruct (L.eq_dec r p) as [eq | _]; [exfalso; apply H0; symmetry; exact eq |].
-      apply TIf; auto.
-      all: apply TSend with (τ := σ); auto.
-    - inversion typ; clear Γ0 H3 Δ0 H4 p0 H0 C1 H2 C2 H6 tau H5 q0 H7 e H1;
-        rename H8 into ltyp1; rename H9 into typC1; rename H10 into typC2.
-      inversion typC1; clear Γ0 H3 Δ0 H4 p0 H0 e H1 C1 H2 C2 H6 tau H5 q0 H7;
-        rename H8 into ltyp2; rename H9 into typC11; rename H10 into typC12.
-      inversion typC2; clear Γ0 H3 Δ0 H4 p0 H0 e H1 C1 H2 C2 H6 tau H5 q0 H7;
-        rename H8 into ltyp3; rename H9 into typC21; rename H10 into typC22.
-      auto with Chor. 
+  Lemma DefSubstTyping : forall (Γ : Loc -> nat -> ExprTyp) (Δ : nat -> Loc * ExprTyp) (C : Chor) (p : Loc) (τ : ExprTyp),
+      Γ ;; (fun n => match n with
+                  | 0 => (p, τ)
+                  | S n => Δ n
+                  end) ⊢c C ::: τ @ p ->
+      ChorSubstTyping Γ (fun n => match n with
+                               | 0 => (p, τ)
+                               | S n => Δ n
+                               end) (DefSubst C) Δ.
+  Proof using.
+    intros Γ Δ C p τ H. unfold ChorSubstTyping; unfold DefSubst.
+    intro n; destruct n; cbn; auto; [|apply TVar].
+    assert (ChorSubstTyping Γ (fun n => match n with
+                                     | 0 => (p, τ)
+                                     | S n0 => Δ n0
+                                     end)
+                            (fun n => match n with
+                                   | 0 => LetGlobal ⟪new⟫ ← C fby C
+                                   | S n0 => Var n0
+                                   end) Δ); [|eapply ChorSubstTypingSpec; eauto].
+    unfold ChorSubstTyping; intro n; destruct n.
+    apply TDefGlobal with (q := p) (σ := τ); auto. apply TVar.
   Qed.
 
   Theorem ChorEquivTyping : forall (C1 C2 : Chor),
       C1 ≡ C2 ->
-      forall (Γ : L.t -> nat -> ExprTyp) (Δ : nat -> L.t * ExprTyp) (τ : ExprTyp) (p : L.t),
-        Γ;; Δ ⊢c C1 ::: τ @ p -> Γ;; Δ ⊢c C2 ::: τ @ p.
-  Proof.
-    intros C1 C2 equiv; induction equiv; intros Γ Δ τ p typ.
-    apply ChorEquiv'Typing with (C1 := C1); auto.
-    apply ChorEquiv'Typing with (C2 := C2) in typ; auto.
-  Qed.
-
+      forall (Γ : Loc -> nat -> ExprTyp) (Δ : nat -> Loc * ExprTyp) (τ : ExprTyp) (p : Loc),
+        Γ ;; Δ ⊢c C1 ::: τ @ p -> Γ ;; Δ ⊢c C2 ::: τ @ p.
+  Proof using.
+    intros C1 C2 equiv; induction equiv; intros Γ Δ τ p typ; auto with Chor;
+      repeat match goal with
+             | [ H : ?Γ ;; ?Δ ⊢c ?C ::: ?t @ ?p |- _ ] =>
+               tryif let x := fresh "_" C in idtac
+               then fail
+               else inversion H; subst; clear H
+             end; auto with Chor.
+    all: repeat match goal with
+                | [IH : forall G D t p, G ;; D ⊢c ?C1 ::: t @ p -> G ;; D ⊢c ?C2 ::: t @ p,
+                     H : ?Γ ;; ?Δ ⊢c ?C1 ::: ?τ @ ?p |- _ ] =>
+                  lazymatch goal with
+                  | [_ : Γ ;; Δ ⊢c C2 ::: τ @ p |- _ ] => fail
+                  | _ => pose proof (IH Γ Δ τ p H)
+                  end
+                end; eauto with Chor.
+    - apply TSend with (τ := τ1); auto.
+      destruct (L.eq_dec l2 l3) as [eq | _ ]; [destruct (H1 eq)|]; auto.
+      apply TSend with (τ := τ0); auto.
+      destruct (L.eq_dec l4 l1) as [eq|_]; [destruct (H0 (eq_sym eq))|]; auto.
+      eapply ChorTypingExt; [| |exact H15]; auto.
+      intros p0 n; cbn; destruct (L.eq_dec l4 p0); destruct (L.eq_dec l2 p0); subst;
+        try match goal with [H : ?a <> ?a |- _] => destruct (H eq_refl) end;
+        auto.
+    - apply TIf. destruct (L.eq_dec l2 l3) as [eq|_]; [destruct (H0 eq)|auto].
+      all: apply TSend with (τ := τ0); auto.
+    - apply TSend with (τ := τ0); auto.
+      apply TIf; auto.
+      destruct (L.eq_dec l3 l1) as [eq | _ ]; [destruct (H0 (eq_sym eq))| auto].
+      rewrite (ExprTypingUnique (Γ l2) e' τ0 τ1 H12 H11); auto.
+  Qed.      
 
   Theorem RelativePreservation :
     (forall (Γ : nat -> ExprTyp) (e : Expr) (τ : ExprTyp),
         Γ ⊢e e ::: τ
         -> forall e' : Expr, ExprStep e e'
                        -> Γ ⊢e e' ::: τ) ->
-    forall (Γ : L.t -> nat -> ExprTyp) (Δ : nat -> L.t * ExprTyp) (C : Chor) (τ : ExprTyp) (p : L.t),
-      Γ;; Δ ⊢c C ::: τ @ p -> forall (R : Redex) (B : list L.t) (C': Chor),
+    forall (Γ : Loc -> nat -> ExprTyp) (Δ : nat -> Loc * ExprTyp) (C : Chor) (τ : ExprTyp) (p : Loc),
+      Γ;; Δ ⊢c C ::: τ @ p -> forall (R : Redex) (B : list Loc) (C': Chor),
         RChorStep R B C C' -> Γ;; Δ ⊢c C' ::: τ @ p.
   Proof.
     intros ExprPreservation Γ Δ C τ p typing; induction typing;
-      intros R B C' step; inversion step; subst; auto.
-    - apply TDone; apply ExprPreservation with (e := e); auto.
-    - apply TSend with (τ := τ); auto; apply ExprPreservation with (e := e); auto.
-    - specialize (IHtyping _ _ _ H8). apply TSend with (τ := τ); auto.
-    - eapply ChorSubstTypingSpec; [apply SendSubstTyping|]; eauto.
-      apply ExprValueTyping with (Γ := Γ p); auto.
-    - apply TIf; auto. apply ExprPreservation with (e := e); auto.
-    - specialize (IHtyping1 _ _ _ H7). specialize (IHtyping2 _ _ _ H8).
-      apply TIf; auto.
+      intros R B C' step; inversion step; subst; clear step; auto.
+    all: repeat match goal with
+                | [ H : ?Γ ⊢e ?e ::: ?τ, H' : ExprStep ?e ?e' |- _ ] =>
+                  lazymatch goal with
+                  | [_ : Γ ⊢e e' ::: τ |- _ ] => fail
+                  | _ => pose proof (ExprPreservation Γ e τ H e' H')
+                  end
+                end; eauto with Chor.
+    - eapply ChorExprSubstTypingSpec; [apply SendExprSubstTyping|]; eauto.
+      eapply ExprValueTyping; eauto.
+    - inversion typing1; subst.
+      eapply ChorExprSubstTypingSpec; [apply SendExprSubstTyping|]; eauto.
     - eapply ChorSubstTypingSpec; [apply DefSubstTyping|]; eauto.
   Qed.
 
-  Theorem ChorValueTyping : forall (C : Chor) (τ : ExprTyp) (p : L.t),
+  Theorem ChorValueTyping : forall (C : Chor) (τ : ExprTyp) (p : Loc),
       ChorVal C ->
        forall Γ1 Γ2 Δ1 Δ2, Γ1;; Δ1 ⊢c C ::: τ @ p -> Γ2;; Δ2 ⊢c C ::: τ @ p.
   Proof.
@@ -285,54 +308,60 @@ Module TypedChoreography (L : Locations) (E : Expression) (TE : TypedExpression 
     apply TDone. eapply ExprValueTyping; eauto.
   Qed.
 
-  Inductive ChorClosedBelow : (L.t -> nat) -> nat -> Chor -> Prop :=
-  | DoneClosedBelow : forall n m p e, ExprClosedBelow (n p) e -> ChorClosedBelow n m (CDone p e)
-  | CVarClosedBelow : forall n m k, k < m -> ChorClosedBelow n m (CVar k)
+  Inductive ChorClosedBelow : (Loc -> nat) -> nat -> Chor -> Prop :=
+  | DoneClosedBelow : forall n m p e, ExprClosedBelow (n p) e -> ChorClosedBelow n m (Done p e)
+  | VarClosedBelow : forall n m k, lt k m -> ChorClosedBelow n m (Var k)
   | SendClosedBelow : forall p e q C n m,
       ExprClosedBelow (n p) e
       -> ChorClosedBelow (fun r => if L.eq_dec q r then S (n q) else n r) m C 
-      -> ChorClosedBelow n m (CSend p e q C)
+      -> ChorClosedBelow n m (Send p e q C)
+  | SyncClosedBelow : forall n m p d q C,
+      ChorClosedBelow n m C -> ChorClosedBelow n m (Sync p d q C)
   | IfClosedBelow : forall n m p e C1 C2,
     ExprClosedBelow (n p) e -> ChorClosedBelow n m C1 -> ChorClosedBelow n m C2
-    -> ChorClosedBelow n m (CIf p e C1 C2)
-  | DefClosedBelow : forall n m C1 C2, ChorClosedBelow n (S m) C1
-                         -> ChorClosedBelow n (S m) C2
-                         -> ChorClosedBelow n m (CDef C1 C2).
-  Lemma ChorClosedBelowTyping : forall (Γ1 Γ2 : L.t -> nat -> ExprTyp)
-                                  (Δ1 Δ2 : nat -> L.t * ExprTyp)
-                                  (C : Chor) (τ : ExprTyp) (p : L.t)
-                                  (n : L.t -> nat) (m : nat),
+    -> ChorClosedBelow n m (If p e C1 C2)
+  | DefLocalClosedBelow : forall n m l C1 C2,
+      ChorClosedBelow n m C1 ->
+      ChorClosedBelow (fun l' => if L.eq_dec l l' then S (n l) else n l') m C2 ->
+      ChorClosedBelow n m (DefLocal l C1 C2)
+  | DefGlobalClosedBelow : forall n m C1 C2,
+      ChorClosedBelow n (S m) C1
+      -> ChorClosedBelow n (S m) C2
+      -> ChorClosedBelow n m (DefGlobal C1 C2).
+
+  Lemma ChorClosedBelowTyping : forall (Γ1 Γ2 : Loc -> nat -> ExprTyp)
+                                  (Δ1 Δ2 : nat -> Loc * ExprTyp)
+                                  (C : Chor) (τ : ExprTyp) (p : Loc)
+                                  (n : Loc -> nat) (m : nat),
       ChorClosedBelow n m C ->
-      (forall (p : L.t) (k : nat), k < (n p) -> Γ1 p k = Γ2 p k) ->
-      (forall k : nat, k < m -> Δ1 k = Δ2 k) ->
+      (forall (p : Loc) (k : nat), lt k (n p) -> Γ1 p k = Γ2 p k) ->
+      (forall k : nat, lt k m -> Δ1 k = Δ2 k) ->
       Γ1;; Δ1 ⊢c C ::: τ @ p -> Γ2;; Δ2 ⊢c C ::: τ @ p.
   Proof.
-    intros Γ1 Γ2 Δ1 Δ2 C; revert Γ1 Γ2 Δ1 Δ2; ChorInduction C;
-      try (rename n into n');
-      intros Γ1 Γ2 Δ1 Δ2 τ q' n m closedC eqΓ eqΔ typ; inversion closedC; inversion typ; subst.
-    - apply TDone; apply ExprClosedBelowTyping with (Γ := Γ1 q') (n := n q'); auto.
+    intros Γ1 Γ2 Δ1 Δ2 C τ p n m cb eqΓ eqΔ typ; revert Γ2 Δ2 n m cb eqΓ eqΔ;
+      induction typ; try rename n into n'; intros Γ2 Δ2 n m cb eqΓ eqΔ;
+        inversion cb; subst.
+    - apply TDone; eapply ExprClosedBelowTyping; [| apply eqΓ|]; eauto.
     - rewrite eqΔ; auto; apply TVar.
-    - apply TSend with (τ := τ0); auto.
-      apply ExprClosedBelowTyping with (Γ := Γ1 p) (n := n p); auto.
-      apply IHC with (Γ1 := fun r n => if L.eq_dec q r then match n with
-                                                          | 0 => τ0
-                                                          | S n0 => Γ1 r n0
-                                                          end else Γ1 r n)
-                     (Δ1 := Δ1) (n := fun r => if L.eq_dec q r then S (n q) else n r) (m := m); auto.
-      intros p3 k lt_k_Sn. destruct (L.eq_dec q p3). destruct k; auto;
-      apply eqΓ. rewrite <- e0. apply Lt.lt_S_n; auto. apply eqΓ; auto.
-    - apply TIf. apply ExprClosedBelowTyping with (Γ := Γ1 p) (n := n p); auto.
-      eapply IHC0; eauto. eapply IHC1; eauto.
-    - apply TDef with (q := q) (σ := σ).
-      eapply IHC0; eauto. intros k lt_k_Sm. simpl. destruct k; auto.
-      apply eqΔ. apply Lt.lt_S_n; auto.
-      eapply IHC1; eauto. intros k lt_k_Sm. simpl. destruct k; auto.
-      apply eqΔ. apply Lt.lt_S_n; auto.
+    - eapply TSend; eauto.
+      eapply ExprClosedBelowTyping; [| | exact H]; eauto.
+      eapply IHtyp; eauto. cbn in *; intros p0 k l.
+      destruct (L.eq_dec q p0); subst; auto. destruct k; auto. apply eqΓ.
+      apply Lt.lt_S_n in l; auto.
+    - apply TIf. eapply ExprClosedBelowTyping; [| apply eqΓ|]; eauto.
+      eapply IHtyp1; eauto. eapply IHtyp2; eauto.
+    - apply TSync; eapply IHtyp; eauto.
+    - eapply TDefLocal. eapply IHtyp1; eauto.
+      eapply IHtyp2; eauto. cbn in *; intros p0 k l.
+      destruct (L.eq_dec p p0); subst; auto. destruct k; auto.
+      apply eqΓ; apply Lt.lt_S_n in l; auto.
+    - eapply TDefGlobal. eapply IHtyp1; eauto. 2: eapply IHtyp2; eauto.
+      all: intros k l; destruct k; auto; apply eqΔ; apply Lt.lt_S_n in l; auto.
   Qed.
 
   Definition ChorClosed := ChorClosedBelow (fun _ => 0) 0.
-  Lemma ChorClosedTyping : forall (Γ1 Γ2 : L.t -> nat -> ExprTyp) (Δ1 Δ2 : nat -> L.t * ExprTyp)
-                             (C : Chor) (τ : ExprTyp)(p : L.t),
+  Lemma ChorClosedTyping : forall (Γ1 Γ2 : Loc -> nat -> ExprTyp) (Δ1 Δ2 : nat -> Loc * ExprTyp)
+                             (C : Chor) (τ : ExprTyp)(p : Loc),
       ChorClosed C -> Γ1;; Δ1 ⊢c C ::: τ @ p -> Γ2;; Δ2 ⊢c C ::: τ @ p.
   Proof.
     intros Γ1 Γ2 Δ1 Δ2 C τ p H H0.
@@ -353,29 +382,29 @@ Module TypedChoreography (L : Locations) (E : Expression) (TE : TypedExpression 
         ExprVal e \/ exists e' : Expr, ExprStep e e') ->
     (forall (v : Expr) (Γ : nat -> ExprTyp),
         Γ ⊢e v ::: bool -> ExprVal v -> {v = tt} + {v = ff}) ->
-    forall (C : Chor) (Γ : L.t -> nat -> ExprTyp) (Δ : nat -> L.t * ExprTyp) (τ : ExprTyp) (p : L.t),
+    forall (C : Chor) (Γ : Loc -> nat -> ExprTyp) (Δ : nat -> Loc * ExprTyp) (τ : ExprTyp) (p : Loc),
       ChorClosed C -> Γ;; Δ ⊢c C ::: τ @ p ->
       ChorVal C \/ exists R C', RChorStep R nil C C'.
   Proof.
-    intros ExprProgress BoolInversion C; ChorInduction C; intros Γ Δ τ q' closedC typ;
-      inversion typ; subst; inversion closedC; subst.
-    2,3,4,5: right.
-    - specialize (ExprProgress _ _ _ H5 H2).
-      destruct ExprProgress as [eval | estep]; [left; apply VDone; auto
-                                               | right; destruct estep as [e' estep]].
-      exists (RDone q' e e');  exists (CDone q' e'); apply DoneEStep; auto.
-    - inversion H2.
-    - specialize (ExprProgress _ _ _ H7 H3); destruct ExprProgress as [eval | estep];
-        [| destruct estep as [e' estep]].
-      -- exists (RSendV p e q);  exists (C [c| ChorIdSubst; SendSubst q e]); auto with Chor.
-      -- exists (RSendE p e e' q);  exists (CSend p e' q C); auto with Chor.
-    - specialize (ExprProgress _ _ _ H7 H4); destruct ExprProgress as [eval | estep];
-        [destruct (BoolInversion _ _ H7 eval) as [ett | eff] |
-         destruct estep as [e' estep]].
-      -- rewrite ett in *; exists (RIfTT p);  exists C0; auto with Chor.
-      -- rewrite eff in *; exists (RIfFF p);  exists C1; auto with Chor.
-      -- exists (RIfE p e e');  exists (CIf p e' C0 C1); auto with Chor.
-    - exists RDef;  exists (C1 [c| DefSubst C0; ExprChorIdSubst]); auto with Chor.
+    intros ExprProgress BoolInversion C Γ Δ τ p cc typ; revert cc; induction typ; intro cc;
+      inversion cc; subst.
+    2: inversion H2.
+    2-6: right.
+    - destruct (ExprProgress e tau (Γ p) ltac:(assumption) ltac:(assumption));
+        [left; constructor; auto | right].
+      destruct H0 as [e' step]; exists (RDone p e e'); exists (Done p e'); auto with Chor.
+    - destruct (ExprProgress e τ (Γ p) ltac:(assumption) ltac:(assumption))
+        as [eval | [e' step]];
+        eexists; eexists; eauto with Chor.
+    - destruct (ExprProgress e bool (Γ p) ltac:(assumption) ltac:(assumption))
+        as [eval | [e' step]];
+        [destruct (BoolInversion e (Γ p) ltac:(assumption) eval); subst|].
+      all: eexists; eexists; eauto with Chor.
+    - eexists; eexists; eauto with Chor.
+    - destruct (IHtyp1 ltac:(assumption)) as [cval | [R [C' step]]].
+      inversion cval; subst. inversion typ1; subst.
+      all: eexists; eexists; eauto with Chor.
+    - exists RDefGlobal; eexists; eauto with Chor.
   Qed.
       
 End TypedChoreography.
