coq/ChoreographyCompiler.v
@@ -1,0 +1,726 @@
+Require Export Expression.
+Require Export Locations.
+Require Export AnnotatedChoreography.
+Require Export PiCalc.
+Require Import LocationMap.
+Require Import LocationSets.
+
+
+Require Import Coq.Arith.Arith.
+Require Import Coq.Program.Wf.
+Require Import Coq.Logic.JMeq.
+Require Import Coq.Classes.RelationClasses.
+Require Import Coq.Lists.List.
+Require Import Sorted Orders Coq.Sorting.Mergesort Permutation.
+Require Import Program.Tactics.
+Require Import Coq.Structures.Orders.
+Require Import Psatz.
+
+From Equations Require Import Equations.
+
+
+Module AChoreographyCompiler (Import E : Expression) (L : Locations) (LM : LocationMap L) (LSorter : LocationSorter L).
+  Include (LocationNotations L).
+  Include ListNotations.
+
+  Module LS := LocationSets L LSorter.
+  Module LF := (LocationFacts L).
+  Module P := (PiCalc E L).
+  Module A := (AnnotatedChoreography E L).
+  Module LMF := (LocationMapFacts L LM).
+    
+  Definition Loc := L.t.
+
+
+  Inductive IProc : Set := (* Intermediate language for process calculus. Can contain partial IChoices *)
+    Skip : IProc (* Skip just exists so that <IProc, MergeIProcs> forms a monoid. This allows me to develop the unbiased version, which is easier to reason about for twist. *)
+  | EndProc : IProc
+  | VarProc : nat -> IProc
+  | DefProc : IProc -> IProc -> IProc
+  | SendProc : Loc -> Expr -> IProc -> IProc
+  | RecvProc : Loc -> IProc -> IProc
+  | EChoiceL : Loc -> IProc -> IProc
+  | EChoiceR : Loc -> IProc -> IProc
+  | IChoiceL : Loc -> IProc -> IProc
+  | IChoiceR : Loc -> IProc -> IProc
+  | IChoiceLR : Loc -> IProc -> IProc -> IProc
+  | IfThenElse : Expr -> IProc -> IProc -> IProc.
+  Hint Constructors IProc : acc.
+  Instance : EqDec Loc := L.eq_dec.
+  Instance : EqDec Expr := ExprEqDec.
+  Definition IProcEqDec : forall P Q : IProc, {P = Q} + {P <> Q}.
+    decide equality.
+    all: try (apply L.eq_dec).
+    apply Nat.eq_dec.
+    all: apply ExprEqDec.
+  Defined.
+  Instance : EqDec IProc := IProcEqDec.
+
+  Ltac IProcInduction x :=
+    let P := fresh "P" in
+    let Q := fresh "Q" in
+    let p := fresh "p" in
+    let e := fresh "e" in
+    let IHP := fresh "IH" P in
+    let IHQ := fresh "IH" Q in
+    let n := fresh "n" in
+    induction x as [| | n | P IHP Q IHQ | p e P IHP | p P IHP | p P IHP | p P IHP | p P IHP | p P IHP | p P IHP Q IHQ | e P IHP Q IHQ].
+  Ltac IProcDestruct x :=
+    let P := fresh "P" in
+    let Q := fresh "Q" in
+    let p := fresh "p" in
+    let e := fresh "e" in
+    let n := fresh "n" in
+    induction x as [| | n | P Q | p e P | p P | p P | p P | p P | p P | p P Q | e P Q].
+  
+  Fixpoint NoPartialIChoices (P : IProc) : Prop :=
+    match P with
+    | Skip => False
+    | EndProc => True
+    | VarProc x => True
+    | DefProc P Q => NoPartialIChoices P /\ NoPartialIChoices Q
+    | SendProc p e P => NoPartialIChoices P
+    | RecvProc p P => NoPartialIChoices P
+    | EChoiceL p P => NoPartialIChoices P
+    | EChoiceR p P => NoPartialIChoices P
+    | IChoiceL p P => False
+    | IChoiceR p P => False
+    | IChoiceLR p P Q => NoPartialIChoices P /\ NoPartialIChoices Q
+    | IfThenElse e P Q => NoPartialIChoices P /\ NoPartialIChoices Q
+    end.
+
+  Fixpoint IProcToProc (P : IProc) : option P.Proc :=
+    match P with
+    | Skip => None
+    | EndProc => Some P.EndProc
+    | VarProc X => Some (P.VarProc X)
+    | DefProc P Q =>
+      match (IProcToProc P) with
+      | Some P' =>
+        match (IProcToProc Q) with
+        | Some Q' => Some (P.DefProc P' Q')
+        | None => None
+        end
+      | None => None
+      end
+    | SendProc p e P =>
+      match IProcToProc P with
+      | Some P' => Some (P.SendProc p e P')
+      | None => None
+      end
+    | RecvProc p P =>
+      match IProcToProc P with
+      | Some P' => Some (P.RecvProc p P')
+      | None => None
+      end
+    | EChoiceL p P =>
+      match IProcToProc P with
+      | Some P' => Some (P.EChoiceL p P')
+      | None => None
+      end
+    | EChoiceR p P =>
+      match IProcToProc P with
+      | Some P' => Some (P.EChoiceR p P')
+      | None => None
+      end
+    | IChoiceL p P => None
+    | IChoiceR p P => None
+    | IChoiceLR p P Q =>
+      match IProcToProc P with
+      | Some P' => match IProcToProc Q with
+                  | Some Q' => Some (P.IChoice p P' Q')
+                  | None => None
+                  end
+      | None => None
+      end
+    | IfThenElse e P Q =>
+      match IProcToProc P with
+      | Some P' => match IProcToProc Q with
+                  | Some Q' => Some (P.IfThenElse e P' Q')
+                  | None => None
+                  end
+      | None => None
+      end
+    end.
+
+  Theorem TotalIProcToProc : forall (P : IProc), NoPartialIChoices P -> IProcToProc P <> None.
+  Proof using.
+    intro x; IProcInduction x; intro npic; cbn in *; try discriminate.
+    all: repeat match goal with
+                | [H : False |- _] => destruct H
+                | [H : ?P, H' : ?P -> ?a <> ?a |- _ ] => exfalso; apply (H' H); auto
+                | [H : ?a <> ?a |- _] => exfalso; apply H; auto
+                | [|- Some _ <> None] => discriminate
+                | [H : ?P /\ ?Q |- _ ] => destruct H
+                | [|- context[IProcToProc ?P]] =>
+                  let iptp := fresh "iptp_" P in
+                  destruct (IProcToProc P) eqn:iptp
+                end.
+  Qed.
+  Corollary TotalIProcToProc_Exists : forall (P : IProc), NoPartialIChoices P -> exists Q : P.Proc, IProcToProc P = Some Q.
+  Proof using.
+    intros P npic; destruct (IProcToProc P) as [Q|] eqn:iptp_P; [exists Q; reflexivity | apply TotalIProcToProc in iptp_P; auto; destruct iptp_P].
+  Qed.
+
+  Fixpoint MergeIProcs (P Q : IProc) : option IProc :=
+    match P with
+    | Skip => Some Q
+    | EndProc =>
+      match Q with
+      | EndProc => Some EndProc
+      | Skip => Some P
+      | _ => None
+      end
+    | VarProc x =>
+      match Q with
+      | VarProc y => if Nat.eq_dec x y then Some (VarProc x) else None
+      | Skip => Some P
+      | _ => None
+      end 
+    | DefProc P1 Q1 =>
+      match Q with
+      | Skip => Some P
+      | DefProc P2 Q2 =>
+        match MergeIProcs P1 P2 with
+        | Some P => match MergeIProcs Q1 Q2 with
+                   | Some Q => Some (DefProc P Q)
+                   | None => None
+                   end
+        | None => None
+        end
+      | _ => None
+      end
+    | SendProc p e P' =>
+      match Q with
+      | Skip => Some P
+      | SendProc q e' Q' =>
+        if L.eq_dec p q
+        then if ExprEqDec e e'
+             then match MergeIProcs P' Q' with
+                  | Some R => Some (SendProc p e R)
+                  | None => None
+                  end
+             else None
+        else None
+      | _ => None
+      end
+    | RecvProc p P' =>
+      match Q with
+      | Skip => Some P
+      | RecvProc q Q' =>
+        if L.eq_dec p q
+        then match MergeIProcs P' Q' with
+             | Some R => Some (RecvProc p R)
+             | _ => None
+             end
+        else None
+      | _ => None
+      end
+    | EChoiceL p P' =>
+      match Q with
+      | Skip => Some P
+      | EChoiceL q Q' =>
+        if L.eq_dec p q
+        then match MergeIProcs P' Q' with
+             | Some R => Some (EChoiceL p R)
+             | None => None
+             end
+        else None
+      | _ => None
+      end
+    | EChoiceR p P' =>
+      match Q with
+      | Skip => Some P
+      | EChoiceR q Q' =>
+        if L.eq_dec p q
+        then match MergeIProcs P' Q' with
+             | Some R => Some (EChoiceR p R)
+             | None => None
+             end
+        else None
+      | _ => None
+      end
+    | IChoiceL p P1 =>
+      match Q with
+      | Skip => Some P
+      | IChoiceL q P2 =>
+        if L.eq_dec p q
+        then match MergeIProcs P1 P2 with
+             | Some R => Some (IChoiceL p R)
+             | None => None
+             end
+        else None
+      | IChoiceR q Q1 =>
+        if L.eq_dec p q
+        then Some (IChoiceLR p P1 Q1)
+        else None
+      | IChoiceLR q P2 Q1 =>
+        if L.eq_dec p q
+        then match MergeIProcs P1 P2 with
+             | Some R => Some (IChoiceLR p R Q1)
+             | None => None
+             end
+        else None
+      | _ => None
+      end
+    | IChoiceR p Q1 =>
+      match Q with
+      | Skip => Some P
+      | IChoiceL q P1 =>
+        if L.eq_dec p q
+        then Some (IChoiceLR p P1 Q1)
+        else None
+      | IChoiceR q Q2 =>
+        if L.eq_dec p q
+        then match MergeIProcs Q1 Q2 with
+             | Some R => Some (IChoiceR p R)
+             | None => None
+             end
+        else None
+      | IChoiceLR q P1 Q2 =>
+        if L.eq_dec p q
+        then match MergeIProcs Q1 Q2 with
+             | Some R => Some (IChoiceLR p P1 R)
+             | None => None
+             end
+        else None
+      | _ => None
+      end      
+    | IChoiceLR p P1 Q1 => 
+      match Q with
+      | Skip => Some P
+      | IChoiceL q P2 =>
+        if L.eq_dec p q
+        then match MergeIProcs P1 P2 with
+             | Some R => Some (IChoiceLR p R Q1)
+             | None => None
+             end
+        else None
+      | IChoiceR q Q2 =>
+        if L.eq_dec p q
+        then match MergeIProcs Q1 Q2 with
+             | Some R => Some (IChoiceLR p P1 R)
+             | None => None
+             end
+        else None
+      | IChoiceLR q P2 Q2 =>
+        if L.eq_dec p q
+        then match MergeIProcs P1 P2 with
+             | Some P => match MergeIProcs Q1 Q2 with
+                        | Some Q => Some (IChoiceLR p P Q)
+                        | None => None
+                        end
+             | None => None
+             end
+        else None
+      | _ => None
+      end
+    | IfThenElse e P1 Q1 =>
+      match Q with
+      | Skip => Some P
+      | IfThenElse e' P2 Q2 =>
+        if ExprEqDec e e'
+        then match MergeIProcs P1 P2 with
+             | Some P => match MergeIProcs Q1 Q2 with
+                        | Some Q => Some (IfThenElse e P Q)
+                        | None => None
+                        end
+             | None => None
+             end
+        else None
+      | _ => None
+      end
+    end.
+  (* Equations MergeIProcs (P Q : IProc) : option IProc := *)
+  (*   { *)
+  (*     MergeIProcs EndProc EndProc := Some EndProc; *)
+  (*     MergeIProcs (VarProc x) (VarProc y) with Nat.eq_dec x y := *)
+  (*       { *)
+  (*       MergeIProcs (VarProc x) (VarProc y) (left eq1) := Some (VarProc x); *)
+  (*       MergeIProcs (VarProc x) (VarProc y) (right neq1) := None *)
+  (*       }; *)
+  (*     MergeIProcs (SendProc p e P) (SendProc q e' Q) with L.eq_dec p q, ExprEqDec e e', MergeIProcs P Q := *)
+  (*       { *)
+  (*       MergeIProcs (SendProc p e P) (SendProc q e' Q) (left eq1) (left eq2) (Some P') := Some (SendProc p e P'); *)
+  (*       MergeIProcs (SendProc p e P) (SendProc q e' Q) (left eq1) (left eq2) None := None; *)
+  (*       MergeIProcs (SendProc p e P) (SendProc q e' Q) (left eq1) (right neq2) _ := None; *)
+  (*       MergeIProcs (SendProc p e P) (SendProc q e' Q) (right neq1) (left neq2) _ := None; *)
+  (*       MergeIProcs (SendProc p e P) (SendProc q e' Q) (right neq1) (right neq2) _ := None *)
+  (*       }; *)
+  (*     MergeIProcs (RecvProc p P) (RecvProc q Q) with L.eq_dec p q, MergeIProcs P Q := *)
+  (*       { *)
+  (*       MergeIProcs (RecvProc p P) (RecvProc q Q) (left eq1) (Some P') := Some (RecvProc p P'); *)
+  (*       MergeIProcs (RecvProc p P) (RecvProc q Q) (left eq1) None := None; *)
+  (*       MergeIProcs (RecvProc p P) (RecvProc q Q) (right neq1) _ := None *)
+  (*       }; *)
+  (*     MergeIProcs (EChoiceL p P) (EChoiceL q Q) with L.eq_dec p q, MergeIProcs P Q := *)
+  (*       { *)
+  (*       MergeIProcs (EChoiceL p P) (EChoiceL q Q) (left eq1) (Some P') := Some (EChoiceL p P'); *)
+  (*       MergeIProcs (EChoiceL p P) (EChoiceL q Q) (left eq1) None := None; *)
+  (*       MergeIProcs (EChoiceL p P) (EChoiceL q Q) (right neq2) _ := None *)
+  (*       }; *)
+  (*     MergeIProcs (EChoiceR p P) (EChoiceR q Q) with L.eq_dec p q, MergeIProcs P Q := *)
+  (*       { *)
+  (*       MergeIProcs (EChoiceR p P) (EChoiceR q Q) (left eq1) (Some P') := Some (EChoiceR p P'); *)
+  (*       MergeIProcs (EChoiceR p P) (EChoiceR q Q) (left eq1) None := None; *)
+  (*       MergeIProcs (EChoiceR p P) (EChoiceR q Q) (right neq1) _ := None *)
+  (*       }; *)
+  (*     MergeIProcs (IChoiceL p P) (IChoiceL q Q) with L.eq_dec p q, MergeIProcs P Q := *)
+  (*       { *)
+  (*       MergeIProcs (IChoiceL p P) (IChoiceL q Q) (left eq1) (Some P') := Some (IChoiceL p P'); *)
+  (*       MergeIProcs (IChoiceL p P) (IChoiceL q Q) (left eq1) None := None; *)
+  (*       MergeIProcs (IChoiceL p P) (IChoiceL q Q) (right neq1) _ := None *)
+  (*       }; *)
+  (*     MergeIProcs (IChoiceR p P) (IChoiceR q Q) with L.eq_dec p q, MergeIProcs P Q := *)
+  (*       { *)
+  (*       MergeIProcs (IChoiceR p P) (IChoiceR q Q) (left eq1) (Some P') := Some (IChoiceR p P'); *)
+  (*       MergeIProcs (IChoiceR p P) (IChoiceR q Q) (left eq1) None := None; *)
+  (*       MergeIProcs (IChoiceR p P) (IChoiceR q Q) (right neq1) _ := None *)
+  (*       }; *)
+  (*     MergeIProcs (IChoiceL p P) (IChoiceR q Q) with L.eq_dec p q := *)
+  (*       { *)
+  (*       MergeIProcs (IChoiceL p P) (IChoiceR q Q) (left eq1) := Some (IChoiceLR p P Q); *)
+  (*       MergeIProcs (IChoiceL p P) (IChoiceR q Q) (right neq1) := None *)
+  (*       }; *)
+  (*     MergeIProcs (IChoiceR p P) (IChoiceL q Q) with L.eq_dec p q := *)
+  (*       { *)
+  (*       MergeIProcs (IChoiceR p P) (IChoiceL q Q) (left eq1) := Some (IChoiceLR p Q P); *)
+  (*       MergeIProcs (IChoiceR p P) (IChoiceL q Q) (right neq1) := None *)
+  (*       }; *)
+  (*     MergeIProcs (IChoiceL p P) (IChoiceLR q P' Q') with L.eq_dec p q, MergeIProcs P P' := *)
+  (*       { *)
+  (*       MergeIProcs (IChoiceL p P) (IChoiceLR q P' Q') (left eq1) (Some P'') := Some (IChoiceLR p P'' Q'); *)
+  (*       MergeIProcs (IChoiceL p P) (IChoiceLR q P' Q') (left eq1) None := None; *)
+  (*       MergeIProcs (IChoiceL p P) (IChoiceLR q P' Q') (right neq1) _ := None *)
+  (*       }; *)
+  (*     MergeIProcs (IChoiceLR p P Q) (IChoiceL q P') with L.eq_dec p q, MergeIProcs P P' := *)
+  (*       { *)
+  (*       MergeIProcs (IChoiceLR p P Q) (IChoiceL q P') (left eq1) (Some P'') := Some (IChoiceLR p P'' Q); *)
+  (*       MergeIProcs (IChoiceLR p P Q) (IChoiceL q P') (left eq1) None := None; *)
+  (*       MergeIProcs (IChoiceLR p P Q) (IChoiceL q P') (right neq1) _ := None *)
+  (*       }; *)
+  (*     MergeIProcs (IChoiceR p Q) (IChoiceLR q P' Q') with L.eq_dec p q, MergeIProcs Q Q' := *)
+  (*       { *)
+  (*       MergeIProcs (IChoiceR p Q) (IChoiceLR q P' Q') (left eq1) (Some Q'') := Some (IChoiceLR p P' Q''); *)
+  (*       MergeIProcs (IChoiceR p Q) (IChoiceLR q P' Q') (left eq1) None := None; *)
+  (*       MergeIProcs (IChoiceR p Q) (IChoiceLR q P' Q') (right neq1) _ := None *)
+  (*       }; *)
+  (*     MergeIProcs (IChoiceLR p P Q) (IChoiceR q Q') with L.eq_dec p q, MergeIProcs Q Q' := *)
+  (*       { *)
+  (*       MergeIProcs (IChoiceLR p P Q) (IChoiceR q Q') (left eq1) (Some Q'') := Some (IChoiceLR p P Q''); *)
+  (*       MergeIProcs (IChoiceLR p P Q) (IChoiceR q Q') (left eq1) None := None; *)
+  (*       MergeIProcs (IChoiceLR p P Q) (IChoiceR q Q') (right neq1) _ := None *)
+  (*       }; *)
+  (*     MergeIProcs (IChoiceLR p P Q) (IChoiceLR q P' Q') with L.eq_dec p q, MergeIProcs P P', MergeIProcs Q Q' := *)
+  (*       { *)
+  (*       MergeIProcs (IChoiceLR p P Q) (IChoiceLR q P' Q') (left eq1) (Some P'') (Some Q'') := Some (IChoiceLR p P'' Q''); *)
+  (*       MergeIProcs (IChoiceLR p P Q) (IChoiceLR q P' Q') (left eq1) _ _ := None; *)
+  (*       MergeIProcs (IChoiceLR p P Q) (IChoiceLR q P' Q') (right neq1) _ _ := None *)
+  (*       }; *)
+  (*     MergeIProcs (IfThenElse e P Q) (IfThenElse e' P' Q') with ExprEqDec e e', MergeIProcs P P', MergeIProcs Q Q' := *)
+  (*       { *)
+  (*       MergeIProcs (IfThenElse e P Q) (IfThenElse e' P' Q') (left eq1) (Some P'') (Some Q'') := Some (IfThenElse e P'' Q''); *)
+  (*       MergeIProcs (IfThenElse e P Q) (IfThenElse e' P' Q') (left eq1) _ _ := None; *)
+  (*       MergeIProcs (IfThenElse e P Q) (IfThenElse e' P' Q') (right neq1) _ _ := None *)
+  (*       }; *)
+  (*     MergeIProcs (DefProc P1 Q1) (DefProc P2 Q2) with MergeIProcs P1 P2, MergeIProcs Q1 Q2 := *)
+  (*       { *)
+  (*       MergeIProcs (DefProc P1 Q1) (DefProc P2 Q2) (Some P) (Some Q) := Some (DefProc P Q); *)
+  (*       MergeIProcs (DefProc P1 Q1) (DefProc P2 Q2) _ _ := None *)
+  (*       }; *)
+  (*     MergeIProcs _ _ := None *)
+  (*   }. *)
+
+  Lemma MergeIProcsComm : forall P Q, MergeIProcs P Q = MergeIProcs Q P.
+  Proof using.
+    intros P; induction P; destruct Q; cbn; auto.
+    all: repeat match goal with
+                | [ H : ?a <> ?a |- _ ] => exfalso; apply H; auto
+                | [ |- ?a = ?a ] => reflexivity
+                | [|- context[Nat.eq_dec ?a ?b]] => destruct (Nat.eq_dec a b); subst; auto
+                | [|- context[L.eq_dec ?a ?b]] => destruct (L.eq_dec a b); LF.LocationOrder; subst; auto
+                | [|- context[ExprEqDec ?a ?b]] => destruct (ExprEqDec a b); LF.LocationOrder; subst; auto
+                | [|- context[MergeIProcs ?a ?b]] => try (let eq := fresh "merge_" a "_" b in destruct (MergeIProcs a b) eqn:eq); simp MergeIProc; cbn; auto
+                | [ IH : forall Q, MergeIProcs ?P Q = MergeIProcs Q ?P, H1 : MergeIProcs ?P ?Q = ?a, H2 : MergeIProcs ?Q ?P = ?b |- _ ] =>
+                  rewrite IH in H1; rewrite H2 in H1; inversion H1; subst; clear H1
+                end.
+  Qed.
+
+  Lemma MergeIProcsInvolutive : forall P, MergeIProcs P P = Some P.
+  Proof using.
+    intro P; induction P; cbn; auto.
+    all: repeat match goal with
+                | [ H : ?a <> ?a |- _ ] => exfalso; apply H; auto
+                | [ |- ?a = ?a ] => reflexivity
+                | [|- context[Nat.eq_dec ?a ?b]] => destruct (Nat.eq_dec a b); subst; auto
+                | [|- context[L.eq_dec ?a ?b]] => destruct (L.eq_dec a b); LF.LocationOrder; subst; auto
+                | [|- context[ExprEqDec ?a ?b]] => destruct (ExprEqDec a b); LF.LocationOrder; subst; auto
+                | [ H : MergeIProcs ?a ?a = Some ?a |- context[MergeIProcs ?a ?a]] => rewrite H; auto
+                end.
+  Qed.
+  Lemma MergeIProcsIdentityL : forall P, MergeIProcs Skip P = Some P.
+  Proof using.
+    intro P; cbn; auto.
+  Qed.
+  Lemma MergeIProcsIdentityR : forall P, MergeIProcs P Skip = Some P.
+  Proof using.
+    destruct P; cbn; auto.
+  Qed.
+    
+  Definition OptionSequence : forall {A B : Type}, (A -> option B) -> option A -> option B :=
+    fun A B f oa => match oa with
+                 | Some a => f a
+                 | None => None
+                 end.
+  Definition OptionSequence2 : forall {A B C : Type}, (A -> B -> option C) -> option A -> option B -> option C :=
+    fun A B C f oa ob => match oa with
+                      | Some a => match ob with
+                                 | Some b => f a b
+                                 | None => None
+                                 end
+                      | None => None
+                      end.
+
+  Inductive MarkedSequence : IProc -> IProc -> IProc -> IProc -> Prop := Mark : forall P Q R S, MarkedSequence P Q R S.
+  Lemma MergeIProcsAssoc : forall P Q R, OptionSequence (MergeIProcs P) (MergeIProcs Q R) = OptionSequence (fun P => MergeIProcs P R) (MergeIProcs P Q).
+  Proof using.
+    intro P; induction P; intros Q R; destruct Q; destruct R; cbn;
+      repeat match goal with
+             | [ |- ?a = ?a ] => reflexivity
+             | [ H : Some _ = None |- _ ] => inversion H
+             | [ H : None = Some _ |- _ ] => inversion H
+             | [ H : Some ?a = Some ?b |- _ ] => inversion H; subst; clear H
+             | [ H1 : ?a = Some _, H2 : ?a = None |- _ ] => rewrite H1 in H2; inversion H2
+             | [ H1 : ?a = Some _, H2 : None = ?a |- _ ] => rewrite H1 in H2; inversion H2
+             | [ H1 : Some _ = ?a, H2 : None = ?a |- _ ] => rewrite <- H1 in H2; inversion H2
+             | [ H1 : Some _ = ?a, H2 : ?a = None |- _ ] => rewrite <- H1 in H2; inversion H2
+             | [ H : ?a <> ?a |- _ ] => destruct (H eq_refl)
+             | [ |- None = Some _ -> _ ] => let H := fresh in intro H; inversion H
+             | [ |- Some ?a = Some ?b -> _ ] => let H := fresh in intro H; inversion H; subst; clear H; cbn
+             | [ |- _ -> Some _ = None -> _ ] => let H := fresh in let H' := fresh in intros H  H'; inversion H'
+             | [ |- _ -> Some ?a = Some ?b -> _ ] => let H := fresh in let H' := fresh in intros H H'; revert H; inversion H'; subst; clear H'
+             | [ |- context[Nat.eq_dec ?a ?b]] => destruct (Nat.eq_dec a b); subst; cbn
+             | [ |- context[L.eq_dec ?a ?b]] => destruct (L.eq_dec a b); subst; cbn
+             | [ |- context[ExprEqDec ?a ?b]] => destruct (ExprEqDec a b); subst; cbn
+             | [ |- context[MergeIProcs ?a ?b]] => let eq := fresh "eq" in destruct (MergeIProcs a b) eqn:eq; cbn
+             (* | [ IH : forall Q R, OptionSequence (MergeIProcs ?P) (MergeIProcs Q R) = OptionSequence (fun S => MergeIProcs S R) (MergeIProcs ?P Q), H : MergeIProcs ?P ?Q = Some ?S, H' : MergeIProcs ?Q ?R = Some ?T, eq1 : MergeIProcs ?S ?R = _, eq2 : MergeIProcs ?P ?T = _ |- _ ] => *)
+             (*   lazymatch goal with *)
+             (*   | [_ : MarkedSequence P Q R S |- _ ] => fail *)
+             (*   | _ => pose proof (Mark P Q R S); let eq := fresh "eq" in pose proof (IH Q R) as eq; rewrite H' in eq; rewrite H in eq; cbn in eq; rewrite eq1 in eq; rewrite eq2 in eq; cbn in eq *)
+             (*   end *)
+             | [ IH : forall Q R, OptionSequence (MergeIProcs ?P) (MergeIProcs Q R) = OptionSequence (fun S => MergeIProcs S R) (MergeIProcs ?P Q), H : MergeIProcs ?P ?Q = _, H' : MergeIProcs ?Q ?R = _ |- _ ] =>
+               lazymatch goal with
+               | [_ : MarkedSequence P Q P Q |- _ ] => fail
+               | _ => pose proof (Mark P Q P Q); let eq := fresh "eq" in pose proof (IH Q R) as eq; rewrite H' in eq; rewrite H in eq; cbn in eq
+               end
+             | [ H : MergeIProcs ?a ?b = MergeIProcs ?c ?d, H' : MergeIProcs ?a ?b = Some _, H'' : MergeIProcs ?c ?d = _ |- _ ] =>
+               rewrite H' in H; rewrite H'' in H; inversion H; subst; clear H
+             | [ H : MergeIProcs ?a ?b = MergeIProcs ?c ?d, H' : MergeIProcs ?a ?b = None, H'' : MergeIProcs ?c ?d = _ |- _ ] =>
+               rewrite H' in H; rewrite H'' in H; inversion H; subst; clear H
+             end.
+  Qed.
+  Corollary MergeIProcsAssoc' : forall P Q R S T, MergeIProcs P Q = Some S -> MergeIProcs Q R = Some T -> MergeIProcs S R = MergeIProcs P T.
+  Proof using.
+    intros P Q R S T H H0; pose proof (MergeIProcsAssoc P Q R) as eq; rewrite H in eq; rewrite H0 in eq; cbn in eq; auto.
+  Qed.
+
+  Fixpoint MergeIProcsList (l : list IProc) : option IProc :=
+    match l with
+    | [] => Some Skip
+    | [P] => Some P
+    | P :: l => OptionSequence (MergeIProcs P) (MergeIProcsList l)
+    end.
+
+  Lemma MergeIProcsList2 : forall P Q, MergeIProcs P Q = MergeIProcsList [P; Q].
+  Proof using.
+    intros P Q; cbn; auto.
+  Qed.
+
+  Fixpoint Deduplicate_ProcList (l : list IProc) : list IProc :=
+    match l with
+    | [] => []
+    | P :: l => if in_dec IProcEqDec P l then Deduplicate_ProcList l else P :: (Deduplicate_ProcList l)
+    end.
+
+  Lemma Deduplicate_In : forall P l, In P l -> In P (Deduplicate_ProcList l).
+  Proof using.
+    intros P l; induction l; cbn; auto; intro i.
+    destruct i as [eq | i]; subst; auto. destruct (in_dec IProcEqDec P l); auto; left; auto.
+    destruct (in_dec IProcEqDec a l); auto; right; auto.
+  Qed.
+    
+  Lemma Deduplicate_In2In : forall P l, In P (Deduplicate_ProcList l) -> In P l.
+  Proof using.
+    intros P l; induction l; cbn; auto; intro i.
+    destruct (in_dec IProcEqDec a l). right; auto. destruct i; auto.
+  Qed.
+  Lemma NoDup_Deduplicate : forall l, NoDup (Deduplicate_ProcList l).
+  Proof using.
+    intro l; induction l; cbn; try (constructor; auto; fail).
+    destruct (in_dec IProcEqDec a l); auto. constructor; auto. intro i; apply n; apply Deduplicate_In2In; auto.
+  Qed.
+
+  Lemma EquivToPerm : forall l l', (forall P, In P l <-> In P l') -> Permutation (Deduplicate_ProcList l) (Deduplicate_ProcList l').
+  Proof using.
+    intros l l' eqv; apply NoDup_Permutation; try (apply NoDup_Deduplicate).
+    intro P; split; intro i; apply Deduplicate_In2In in i; apply eqv in i; apply Deduplicate_In in i; auto.
+  Qed.
+
+  Lemma MergeIProcsListPerm : forall l l', Permutation l l' -> MergeIProcsList l = MergeIProcsList l'.
+  Proof using.
+    intros l l' perm; induction perm; auto; cbn.
+    - destruct l. apply Permutation_nil in perm; subst; auto. destruct l'. apply Permutation_sym in perm; apply Permutation_nil_cons in perm; destruct perm.
+      rewrite IHperm; auto.
+    - destruct l; cbn. apply MergeIProcsComm.
+      destruct (match l with
+                | [] => Some i
+                | _ :: _ => OptionSequence (MergeIProcs i) (MergeIProcsList l)
+                end); cbn; auto.
+      pose proof (MergeIProcsAssoc x y i0).
+      pose proof (MergeIProcsAssoc y x i0).
+      rewrite MergeIProcsComm with (P := y) (Q := x) in H0. rewrite <- H0 in H. rewrite H. reflexivity.
+    - transitivity (MergeIProcsList l'); auto.
+  Qed.
+
+  Lemma MergeIProcsIn : forall P l, In P l -> MergeIProcsList (P :: l) = MergeIProcsList l.
+  Proof using.
+    intros P l; revert P; induction l as [| Q l]; intros P i; cbn; [inversion i|].
+    destruct l; [cbn; destruct i as [eq|i]; [|inversion i]; subst; apply MergeIProcsInvolutive|].
+    destruct i as [eq|i]; subst; cbn; destruct (match l with
+                                                | [] => Some i0
+                                                | _ :: _ => OptionSequence (MergeIProcs i0) (MergeIProcsList l)
+                                                end) eqn:eq; cbn; auto.
+    rewrite (MergeIProcsAssoc P P i); rewrite MergeIProcsInvolutive; cbn; auto.
+    pose proof (IHl P i) as H; cbn in H. rewrite eq in H.
+    rewrite MergeIProcsComm with (P := Q) (Q := i1).
+    rewrite (MergeIProcsAssoc P i1 Q). cbn in H. rewrite H. cbn. reflexivity.
+  Qed.
+    
+
+  Lemma MergeIProcsDeduplicate : forall l, MergeIProcsList l = MergeIProcsList (Deduplicate_ProcList l).
+  Proof using.
+    intro l; induction l; cbn; auto.
+    destruct (in_dec IProcEqDec a l); cbn.
+    destruct l; [inversion i |rewrite <- IHl; apply MergeIProcsIn in i; rewrite <- i at 2; auto].
+    rewrite <- IHl.
+    destruct l. cbn; auto.
+    destruct (Deduplicate_ProcList (i :: l)) eqn:eq. assert (In i []) as H by (rewrite <- eq; apply Deduplicate_In; left; auto); inversion H.
+    reflexivity.
+  Qed.
+
+  Corollary MergeIProcsEquiv : forall l l', (forall P, In P l <-> In P l') -> MergeIProcsList l = MergeIProcsList l'.
+  Proof using.
+    intros l l' H; rewrite MergeIProcsDeduplicate; rewrite (MergeIProcsDeduplicate l'); apply MergeIProcsListPerm; apply EquivToPerm; auto.
+  Qed.
+
+  Lemma MergeIProcsApp : forall l l', (OptionSequence2 MergeIProcs) (MergeIProcsList l) (MergeIProcsList l') = MergeIProcsList (l ++ l').
+  Proof using.
+    intro l; induction l as [|P l]; cbn; intro l'.
+    destruct (MergeIProcsList l'); auto.
+    rewrite <- IHl.
+    destruct (l ++ l') eqn:eq. apply app_eq_nil in eq; destruct eq; subst; cbn; rewrite MergeIProcsIdentityR; reflexivity.
+    destruct l; cbn in eq; subst. rewrite IHl. rewrite app_nil_l. destruct (MergeIProcsList (i :: l0)); cbn; auto.
+    inversion eq; subst; clear eq. cbn. destruct (match l with | [] => Some i | _ :: _ => OptionSequence (MergeIProcs i) (MergeIProcsList l) end); cbn; auto.
+    destruct (MergeIProcsList l'); cbn.
+    rewrite (MergeIProcsAssoc P i0 i1). destruct (MergeIProcs P i0); cbn; reflexivity.
+    destruct (MergeIProcs P i0); cbn; reflexivity.
+  Qed.
+       
+  Lemma MergeIProcsTwist : forall P1 P2 Q1 Q2, (OptionSequence2 MergeIProcs) (MergeIProcs P1 Q1) (MergeIProcs P2 Q2) = (OptionSequence2 MergeIProcs) (MergeIProcs P1 P2) (MergeIProcs Q1 Q2).
+  Proof using.
+    intros P1 P2 Q1 Q2. repeat rewrite MergeIProcsList2. repeat rewrite MergeIProcsApp. apply MergeIProcsListPerm.
+    cbn; repeat constructor; auto; fail.
+  Qed.
+
+  Equations ProjectAChor (C: A.Chor) (l : Loc) (Env : Loc) : option IProc :=
+    {
+      ProjectAChor (A.Done p e) l Env with L.eq_dec p l :=
+        {
+        ProjectAChor (A.Done p e) l Env (left eq1) := Some (SendProc Env e EndProc);
+        ProjectAChor (A.Done p e) l Env (right neq) := Some EndProc
+        };
+      ProjectAChor (A.Var x) _ _ := Some (VarProc x);
+      ProjectAChor (A.Send p e q C) l Env with L.eq_dec p l, L.eq_dec q l, ProjectAChor C l Env :=
+        {
+        ProjectAChor (A.Send p e q C) l Env (left eq1) (right neq) (Some P) := Some (SendProc q e P);
+        ProjectAChor (A.Send p e q C) l Env (right neq) (left eq1) (Some P) := Some (RecvProc p P);
+        ProjectAChor (A.Send p e q C) l Env _ _ _ := None
+        };
+      ProjectAChor (A.If n p e C1 C2) l Env with L.eq_dec p l, ProjectAChor C1 l Env, ProjectAChor C2 l Env :=
+        {
+        ProjectAChor (A.If n p e C1 C2) l Env (left eq1) (Some P) (Some Q) := Some (IfThenElse e P Q);
+        ProjectAChor (A.If n p e C1 C2) l Env (right neq) (Some P) (Some Q) := MergeIProcs P Q;
+        ProjectAChor (A.If n p e C1 C2) l Env _ _ _ := None
+        };
+      ProjectAChor (A.Sync p d q C) l Env with L.eq_dec p l, L.eq_dec q l, ProjectAChor C l Env :=
+        {
+        ProjectAChor (A.Sync p d q C) l Env (left eq1) (right neq) (Some P) := 
+          match d with
+          | A.LChoice => Some (EChoiceL q P)
+          | A.RChoice => Some (EChoiceR q P)
+          end;
+        ProjectAChor (A.Sync p d q C) l Env (right neq) (left eq2) (Some P) :=
+          match d with
+          | A.LChoice => Some (IChoiceL q P)
+          | A.RChoice => Some (IChoiceR q P)
+          end;
+        ProjectAChor (A.Sync p d q C) l Env (right neq) (right neq) (Some P) := Some P;
+        ProjectAChor (A.Sync p d q C) l Env _ _ _ := None
+        };
+      ProjectAChor (A.Def C1 C2) l Env with ProjectAChor C1 l Env, ProjectAChor C2 l Env :=
+        {
+        ProjectAChor (A.Def C1 C2) l Env (Some P) (Some Q) := Some (DefProc P Q);
+        ProjectAChor (A.Def C1 C2) l Env _ _ := None
+        }
+    }.
+  Inductive MarkedProjection : A.Chor -> Loc -> Loc -> Prop := MarkProj : forall C l Env, MarkedProjection C l Env.
+  Theorem ProjectAChorEquiv' : forall (C C' : A.Chor) (l : Loc) (Env : Loc), A.chorEquiv' C C' -> ProjectAChor C l Env = ProjectAChor C' l Env.
+  Proof using.
+    intros C C' l Env equiv; revert l Env; induction equiv; intros l' Env; simp ProjectAChor;
+      repeat (match goal with
+              | [ H : ?a <> ?a |- _ ] => destruct (H eq_refl)
+              | [ |- ?a = ?a ] => reflexivity
+              | [ H : ?a = Some _, H2 : ?a = None |- _ ] => rewrite H in H2; inversion H2
+              | [ H1 : ?a = Some ?b, H2 : ?a = Some ?c |- _ ] =>
+                (unify b c) + (rewrite H1 in H2; inversion H2; subst; clear H2)
+              | [ |-context[ExprEqDec ?a ?b]]=> destruct (ExprEqDec a b); subst; cbn; auto
+              | [ |-context[L.eq_dec ?a ?b]]=> destruct (L.eq_dec a b); LF.LocationOrder; subst; cbn; auto
+              | [ |-context[Nat.eq_dec ?a ?b]] => destruct (Nat.eq_dec a b); subst; cbn; auto
+              | [ |-context[MergeIProcs ?a ?b]] =>
+                lazymatch goal with
+                | [ H : MergeIProcs a b = _ |- _ ] => rewrite H
+                | _ => let eq := fresh "merge_" a "_" b in destruct (MergeIProcs a b) eqn:eq; auto; cbn
+                end
+              | [ |-context[ProjectAChor ?a ?b]] => let eq := fresh "eq_project_" a "_" b in destruct (ProjectAChor a b) eqn:eq; auto; cbn
+              | [ d : A.LRChoice |- _] =>
+                match goal with
+                | [ |- context[d]] => destruct d; cbn
+                end
+              | [ IH : forall l E, ProjectAChor ?C1 l E = ProjectAChor ?C2 l E, H : ProjectAChor ?C1 ?l ?E = _ , H2 : ProjectAChor ?C2 ?l ?E = _ |- _ ] =>
+                lazymatch goal with
+                | [ _ : MarkedProjection C1 l E |- _ ] => fail
+                | _ => pose proof (MarkProj C1 l E); let eq := fresh "eq_" IH in pose proof (IH l E) as eq; rewrite H in eq; rewrite H2 in eq; inversion eq; subst
+                end
+              end; simp ProjectAChor).
+    all: repeat match goal with
+           | [ H : ?a = ?a |- _ ] => clear H
+           | [ H : MarkedProjection _ _ _ |- _ ] => clear H
+           end.
+    - pose proof (MergeIProcsTwist i10 i7 i9 i6). rewrite merge_i10_i9 in H0. rewrite merge_i3_i2 in H0. rewrite merge_i7_i6 in H0. rewrite merge_i0_i in H0. cbn in H0.
+      rewrite merge_i11_i8 in H0; rewrite merge_i4_i1 in H0; auto.
+    - pose proof (MergeIProcsTwist i10 i7 i9 i6). rewrite merge_i10_i9 in H0. rewrite merge_i3_i2 in H0. rewrite merge_i7_i6 in H0. rewrite merge_i0_i in H0. cbn in H0.
+      rewrite merge_i11_i8 in H0; rewrite merge_i4_i1 in H0; auto.
+    - pose proof (MergeIProcsTwist i10 i7 i9 i6). rewrite merge_i10_i9 in H0. rewrite merge_i3_i2 in H0. rewrite merge_i7_i6 in H0. rewrite merge_i0_i in H0. cbn in H0.
+      rewrite merge_i4_i1 in H0; auto.
+    - pose proof (MergeIProcsTwist i0 i6 i3 i7). rewrite merge_i0_i in H0. rewrite merge_i3_i2 in H0. rewrite MergeIProcsComm with (P := i6) (Q := i7) in H0. rewrite merge_i7_i6 in H0.
+      cbn in H0. rewrite MergeIProcsComm with (P := i1) (Q := i4) in H0. rewrite merge_i4_i1 in H0. destruct (MergeIProcs i0 i3); cbn in H0; inversion H0.
+    - pose proof (MergeIProcsTwist i8 i5 i9 i6). rewrite merge_i0_i in H0. rewrite merge_i3_i2 in H0. rewrite (MergeIProcsComm i8 i9) in H0. rewrite merge_i9_i8 in H0.
+      rewrite (MergeIProcsComm i5 i6) in H0; rewrite merge_i6_i5 in H0. cbn in H0. rewrite merge_i10_i7 in H0. rewrite (MergeIProcsComm i1 i4) in H0; rewrite merge_i4_i1 in H0.
+      inversion H0.
+    - pose proof (MergeIProcsTwist i4 i7 i5 i8). rewrite (MergeIProcsComm i4 i7) in H0; rewrite merge_i0_i in H0. rewrite (MergeIProcsComm i5 i8) in H0; rewrite merge_i3_i2 in H0.
+      rewrite (MergeIProcsComm i4 i5) in H0; rewrite merge_i5_i4 in H0. rewrite (MergeIProcsComm i7 i8) in H0; rewrite merge_i8_i7 in H0. cbn in H0.
+      rewrite (MergeIProcsComm i6 i9) in H0; rewrite merge_i9_i6 in H0. inversion H0.
+    - pose proof (MergeIProcsTwist i2 i1 i5 i4). rewrite (MergeIProcsComm i1 i4) in H0; rewrite merge_i0_i in H0. rewrite merge_i2_i1 in H0; rewrite merge_i5_i4 in H0. cbn in H0.
+      rewrite (MergeIProcsComm i3 i6) in H0; rewrite merge_i6_i3 in H0. destruct (MergeIProcs i2 i5); cbn in H0; inversion H0.
+  Qed.
+End AChoreographyCompiler.
